\documentclass[11pt]{article}
\usepackage{graphicx}
\usepackage[utf8]{inputenc} 
\usepackage{amsmath}
\usepackage{cancel}
\usepackage{bbold}
\usepackage{color}
\usepackage{amsfonts}
\usepackage{mathtools}
\usepackage{braket}


\begin{document}
\title{FYS3110 Midterm exam}
\author{Ingrid A V Holm}
\maketitle


\section{Problem 2}

\begin{flushleft}
We have:

\begin{equation}
\ket{\psi(s)} \equiv e^{-\hat{H}s} \ket{\psi}
\end{equation}

If $s= \frac{it}{\hbar}$ this would be the time propagator. However, $s$ is \textit{real}. We can expand $e^{-Hs}$ to get $\ket{\psi(s)}$:

$$
\ket{\psi(s)} =
e^{-\hat{H}s}
\ket{\psi}
= (1 + s \hat{H} + \frac{s^2}{2!} \hat{H} \hat{H} + \frac{s^3}{3!} \hat{H} \hat{H} \hat{H} + ...) \ket{\psi}
$$
\end{flushleft}

MOVE DOWN WHEN FINISHED


\section{Problem 1} \begin{flushleft}
This problem is about spin-$1/2$ systems, where for a singel spin-$1/2$ we have the simultaneous orthonormal eigenstates of the spin squared operator $\hat{S}^2$ and spin z-component $\hat{S}_z$:

\begin{equation}
\hat{S}^2 = \hat{S}_x^2 + \hat{S}_y^2 + \hat{S}_z^2
\end{equation}

\begin{equation}
\ket{\uparrow} \equiv
\ket{s= \frac{1}{2} \text{, } m_s = + \frac{1}{2}} \text{ ; } \ket{\downarrow} \equiv
\ket{s= \frac{1}{2} \text{, } m_s = - \frac{1}{2}}
\end{equation}

And we have:

\begin{equation}
\hat{S}^2 \ket{m_s = \pm\frac{1}{2} }  = \frac{\hbar^2}{2} \ket{m_s = \pm \frac{1}{2}}
\end{equation}

\begin{equation}
\hat{S}_z \ket{\uparrow} = +\frac{\hbar}{2} \ket{\uparrow} \text{ ; }
\hat{S}_z \ket{\downarrow} = -\frac{\hbar}{2} \ket{\downarrow}
\end{equation}

We also have the commutation relations

\begin{equation}
[ \hat{S}_x, \hat{S}_y ] = i \hbar \hat{S}_z \text{ , } [ \hat{S}_y, \hat{S}_z ] = i \hbar \hat{S}_x \text{ , }
[ \hat{S}_z, \hat{S}_x ] = i \hbar \hat{S}_y
\end{equation}

In addition we have the lowering and raising operators:

\begin{equation}
\hat{S}_{\pm} = \hat{S}_x \pm i \hat{S}_y
\end{equation}
\end{flushleft}

\pagebreak
\subsection{}

\begin{flushleft}
We wish to show that $\hat{S}_+ \ket{\downarrow}$ is an eigenstate of $\hat{S}_z$. In advance, we know that $\hat{S}_+$ is the raising operator, which raises $m_s$ by one (in this case $m_s \rightarrow +\frac{1}{2}$), so this \textit{should } give an eigenstate.
\end{flushleft}

\begin{flushleft}
We begin by finding the commutation relation $[\hat{S}_z, \hat{S}_+]$:

$$
[\hat{S}_z, \hat{S}_+] = \hat{S}_z \hat{S}_+ - \hat{S}_+ \hat{S}_z = \hat{S}_z (\hat{S}_x + i \hat{S}_y) - (\hat{S}_x + i \hat{S}_y) \hat{S}_z = [\hat{S}_z, \hat{S}_x] - i [\hat{S}_y, \hat{S}_z]
$$

$$
[\hat{S}_z, \hat{S}_+] = i \hbar \hat{S}_y - i \cdot i \hbar \hat{S}_x = \hbar (\hat{S}_x + i \hat{S}_y) = \hbar \hat{S}_+
$$

Now we use this in the expression

$$
\hat{S}_z ( \hat{S}_+ \ket{\downarrow}) = (\hat{S}_+\hat{S}_z +\hbar \hat{S}_+) \ket{\downarrow} = \hat{S}_+\hat{S}_z \ket{\downarrow} +\hbar \hat{S}_+ \ket{\downarrow} = ( - \frac{\hbar}{2} + \hbar) \hat{S}_+ \ket{\downarrow} = +\frac{ \hbar}{2} \hat{S}_+ \ket{\downarrow}
$$


So $\hat{S}_+ \ket{\downarrow}$ is an eigenstate of $\hat{S}_z$ with eigenvalue $+ \frac{\hbar}{2}$. We know that this is the eigenvalue of $\ket{\uparrow}$. 
\end{flushleft}


\subsection{}

\begin{flushleft}
We wish to express $\hat{S}_- \hat{S}_+$ in terms of $\hat{S}_z$ and $\hat{S}^2$.

$$
\hat{S}_- \hat{S}_+ = (\hat{S}_x - i \hat{S}_y)(\hat{S}_x + i \hat{S}_y) = \hat{S}_x^2 + \hat{S}_y^2 + i(\hat{S}_x \hat{S}_y - \hat{S}_y \hat{S}_x) 
$$

$$
\hat{S}_- \hat{S}_+ = \hat{S}^2 - \hat{S}_z^2 + i[\hat{S}_x, \hat{S}_y] = \hat{S}^2 - \hat{S}_z^2 - \hbar \hat{S}_z
$$
\end{flushleft}

\begin{flushleft}
Find the norm of $\ket{\psi_{1,2}} = \hat{S}_+ \ket{\downarrow,\uparrow}$, using that $\hat{S}_+^{\dagger} = \hat{S}_-$ and $\ket{\downarrow,\uparrow}$ is orthonormal: 

$$
|\braket{\psi_{1,2}|\psi_{1,2}}| = |(\hat{S}_+ \ket{\downarrow,\uparrow})^{\dagger} \hat{S}_+ \ket{\downarrow, \uparrow}| = |\bra{\downarrow, \uparrow} \hat{S}_- \hat{S}_+ \ket{\downarrow, \uparrow}|
$$

$$
|\braket{\psi_{1,2}|\psi_{1,2}}| = |\bra{\downarrow, \uparrow} (\hat{S}^2 - \hat{S}_z^2 - \hbar \hat{S}_z) \ket{\downarrow, \uparrow}|
$$

Now we do $\psi_1$ and $\psi_2$ separately: 


$$
|\braket{\psi_1|\psi_1}|= |\bra{\downarrow} (\frac{\hbar^2}{2} - \frac{\hbar^2}{4} + \hbar \frac{\hbar}{2}) \ket{\downarrow}| = |\frac{3\hbar^2}{4} \braket{\uparrow|\uparrow}|
$$

$$
|\braket{\psi_2|\psi_2}|= |\bra{\uparrow} (\frac{\hbar^2}{2} - \frac{\hbar^2}{4} - \hbar \frac{\hbar}{2}) \ket{\uparrow}| = |-\frac{\hbar^2}{4} \braket{\uparrow|\uparrow}| = \frac{\hbar^2}{4}
$$

The norms are $\ket{\psi_1} = \sqrt{|\braket{\psi_1|\psi_1}|} = \frac{\sqrt{3} \hbar}{2}$; $\ket{\psi_2} = \sqrt{|\braket{\psi_2|\psi_2}|} = \frac{ \hbar}{2}$ .
\end{flushleft}

\subsection{}

\begin{flushleft}
We now have that

\begin{equation}
\hat{S}_+ \ket{\downarrow} = \hbar \ket{\uparrow} \text{ , } \hat{S}_- \ket{\uparrow} = \hbar \ket{\downarrow}
\end{equation}
\end{flushleft}

\begin{flushleft}
We consider $\ket{\phi} = \frac{1}{\sqrt{2}} \big( 
\ket{\uparrow} + e^{i \theta} \ket{\downarrow}
\big)$ where $\theta$ is real. Notice that the probability of $\ket{\downarrow}$ is $|\frac{1}{\sqrt{2}} e^{i\theta}|^2 = \frac{1}{2} e^{i \theta} e^{-i \theta} = \frac{1}{2}$. We want to find the \textit{uncertainty product} $\sigma_{sx}^2 \sigma_{sy}^2$, where:

\begin{equation}
\sigma_{sx}^2 = \bra{\phi} \Big( 
\hat{S}_x - \bra{\phi}\hat{S}_x \ket{\phi}
\Big)^2
\ket{\phi} 
\end{equation}

\begin{equation}
\sigma_{sy}^2 = \bra{\phi} \Big( 
\hat{S}_y - \bra{\phi}\hat{S}_y \ket{\phi}
\Big)^2
\ket{\phi}
\end{equation}

Fin expressions for $\hat{S}_x$ and $\hat{S}_y$:

$$
\hat{S}_+ + \hat{S}_- = (\hat{S}_x + i \hat{S}_y) + (\hat{S}_x - i \hat{S}_y) = 2 \hat{S}_x \rightarrow \hat{S}_x = \frac{1}{2} (\hat{S}_+ + \hat{S}_-)
$$

$$
\hat{S}_+ - \hat{S}_- = (\hat{S}_x + i \hat{S}_y) - (\hat{S}_x - i \hat{S}_y) = 2 i\hat{S}_y \rightarrow \hat{S}_y = \frac{1}{2i} (\hat{S}_+ - \hat{S}_-)
$$

We can now find the inner products in $\sigma$, assuming that $\hat{S}_+ \ket{\uparrow} = 0$, $\hat{S}_- \ket{\downarrow} = 0$:

$$
\bra{\phi} \hat{S}_x \ket{\phi} = \frac{1}{2} \bra{\phi} (\hat{S}_+ + \hat{S}_-) \ket{phi} = \frac{1}{2} \bra{\phi} (\hat{S}_+ + \hat{S}_-) 
\frac{1}{\sqrt{2}} \big( 
\ket{\uparrow} + e^{i \theta} \ket{\downarrow}
\big)
$$

$$
= \frac{1}{2} \frac{1}{\sqrt{2}} \big( 
\bra{\uparrow} + e^{-i \theta} \bra{\downarrow}
\big) 
\frac{1}{\sqrt{2}}
(\hbar e^{i \theta} \ket{\uparrow} + \hbar \ket{\downarrow})
= \frac{1}{4} \hbar (e^{i \theta} + e^{-i \theta}) = \frac{\hbar
}{2} \cos \theta
$$

$$
\bra{\phi} \hat{S}_y \ket{\phi} 
= \frac{1}{2i} \bra{\phi} (\hat{S}_+ - \hat{S}_-) \ket{\phi} 
= \frac{1}{2i} \bra{\phi} (\hat{S}_+ - \hat{S}_-) 
\frac{1}{\sqrt{2}} \big( 
\ket{\uparrow} + e^{i \theta} \ket{\downarrow}
\big)
$$

$$
= \frac{1}{2i} \frac{1}{\sqrt{2}} \big( 
\bra{\uparrow} + e^{-i \theta} \bra{\downarrow}
\big) 
\frac{1}{\sqrt{2}}
(\hbar e^{i \theta} \ket{\uparrow} - \hbar \ket{\downarrow})
= \frac{1}{4i} \hbar (e^{i \theta} - e^{-i \theta}) = \frac{\hbar
}{2} \sin \theta
$$


\end{flushleft}




























\end{document}